intermediate/Veritas.Intermediate.Verify.fsti
@@ -314,7 +314,22 @@ val lemma_verifiable_implies_prefix_verifiable
   Lemma (ensures (let li = prefix l i in
                   verifiable vsinit li))
         [SMTPat (verifiable vsinit (prefix l i))]
-  
+
+val lemma_addm_props (#vcfg:_)
+                     (vs:vtls vcfg{Valid? vs})
+                     (e:logS_entry _{AddM_S? e}):
+  Lemma (requires (Valid? (verify_step vs e)))
+        (ensures (let AddM_S s (k,v) s' = e in
+                  let st' = thread_store vs in
+                  inuse_slot st' s' /\
+                  (let k' = stored_key st' s' in
+                   is_proper_desc k k' /\
+                   is_merkle_key k' /\
+                   (let mv' = to_merkle_value (stored_value st' s') in
+                    let d = desc_dir k k' in
+                    (mv_points_to_none mv' d || 
+                     is_desc (mv_pointed_key mv' d) k)))))
+
 (* verifiability implies consistency of the log *)
 val lemma_verifiable_implies_consistent_log (#vcfg:_) (vsinit: vtls vcfg) (l: logS _{verifiable vsinit l}):
   Lemma (ensures (let st = thread_store vsinit in
@@ -424,21 +439,6 @@ val lemma_vaddm_preserves_ismap_new_key
                      let AddM_S _ (k,_) _ = e in
                      not (store_contains_key st k)))
           (ensures (Valid? (verify_step vs e) ==> S.is_map (thread_store (verify_step vs e))))
-
-val lemma_addm_props (#vcfg:_)
-                     (vs:vtls vcfg{Valid? vs})
-                     (e:logS_entry _{AddM_S? e}):
-  Lemma (requires (Valid? (verify_step vs e)))
-        (ensures (let AddM_S s (k,v) s' = e in
-                  let st = thread_store vs in
-                  inuse_slot st s' /\
-                  (let k' = stored_key st s' in
-                   is_proper_desc k k' /\
-                   is_merkle_key k' /\
-                   (let mv' = to_merkle_value (stored_value st s') in
-                    let d = desc_dir k k' in
-                    (mv_points_to_none mv' d || 
-                     is_desc (mv_pointed_key mv' d) k)))))
 
 (* addb preserves spec relationship if the kew is not in store *)
 val lemma_vaddb_preserves_spec_new_key
