intermediate/Veritas.Intermediate.Store.fsti
@@ -264,7 +264,7 @@ val mevict_from_store
 
                           // nothing changes in slot s', except it points to none in directoin d
                           inuse_slot st' s' /\
-                          stored_key st' s' = stored_key st s /\
+                          stored_key st' s' = stored_key st s' /\
                           stored_value st' s' = stored_value st s' /\
                           add_method_of st' s' = add_method_of st s' /\
                           points_to_info st' s' od = points_to_info st s' od /\
